Making something work in the basic cases

Clap/Test/Compiler/Traverse/Down.lean
@@ -18,13 +18,89 @@ set_option Clap.traversalDbg true in
 set_option trace.Clap.Compile.dbg true in
 #eval runTest ``testInnerReturn
 
+def testRightBind : Option ℕ := do
+  let x ← F 1
+  let y ← F (x + 10)
+  return y
+set_option trace.Clap.Compile true in
+set_option Clap.traversalDbg true in
+set_option trace.Clap.Compile.dbg true in
+#eval runTest ``testRightBind
+
+def testLeftBind : Option ℕ := do
+  let y ← F ((←do
+    let x ← F 1;
+    return x) + 10
+  )
+  return y
+set_option trace.Clap.Compile true in
+set_option Clap.traversalDbg true in
+set_option trace.Clap.Compile.dbg true in
+#eval runTest ``testLeftBind
+
+def testTreeBind : Option ℕ := do
+  let y ← F ((←do
+    let x ← F 1;
+    let y ← F (x + 10)
+    return y) + 100
+  )
+  let z ← F ((←do
+    let x ← F 1000;
+    let y ← F (x + 10000)
+    return y) + 100000
+  )
+  return y + z
+
+def flattenedTreeBind : Option ℕ := do
+  let x ← F 1
+  let y ← F (x + 10)
+  let y ← F (y + 100)
+  let x ← F 1000
+  let y' ← F (x + 10000)
+  let z ← F (y' + 100000)
+  y + z
+
+example :
+  testTreeBind =
+  (((F 1).bind fun x => (F (x.add 10)).bind fun y => some y).bind fun __do_lift =>
+    (F (__do_lift.add 100)).bind fun y =>
+      ((F 1000).bind fun x => (F (x.add 10000)).bind fun y => some y).bind fun __do_lift =>
+        (F (__do_lift.add 100000)).bind fun z => some (y.add z))
+:=
+  rfl
+  -- by
+  -- unfold testTreeBind
+  -- unfold_projs
+
+example :
+  testTreeBind = flattenedTreeBind
+:= by
+  simp only [
+    testTreeBind,
+    flattenedTreeBind
+  ]
+  simp only [
+    bind_assoc
+  ]
+  rfl
+
+
+#print testTreeBind
+set_option trace.Clap.Compile true in
+set_option Clap.traversalDbg true in
+set_option trace.Clap.Compile.dbg true in
+#eval runTest ``testTreeBind
 
 def exex' : Option ℕ := do
   let z ← F 2
   let x ← H 4
   let y ← (do let x ← G (x + z); let y ← G x; H (x + z))
   H y
-#eval exex' == F 8
+#check @Option.bind_assoc
+set_option trace.Clap.Compile true in
+set_option Clap.traversalDbg true in
+set_option trace.Clap.Compile.dbg true in
+#eval runTest ``exex'
 
 def exex'' : Option ℕ := do
   let z ← F 2
